Labb2/testStuff.dfy
@@ -1,0 +1,17 @@
+predicate p2(a : seq<int>, b : seq<int>)
+{
+    forall i :: 0 < i < |a| ==> Count(a[i],a) == Count(a[i],b)
+}
+
+function Count(val : int, s : seq<int>) : int
+{
+  if |s| == 0 then 0 else
+  if val == s[0] then Count(val, s[1..]) else Count(val, s[1..])
+}
+
+method Main()
+{
+    var s1 := [1,2,2,3,4];
+    var s2 := [1,3,4,2,2];
+    assert p2(s1,s2);
+}
